@prefix : <http://www.vberg.dev/ontologies/kinship#> .
@prefix owl: <http://www.w3.org/2002/07/owl#> .
@prefix rdf: <http://www.w3.org/1999/02/22-rdf-syntax-ns#> .
@prefix xml: <http://www.w3.org/XML/1998/namespace> .
@prefix xsd: <http://www.w3.org/2001/XMLSchema#> .
@prefix rdfs: <http://www.w3.org/2000/01/rdf-schema#> .
@prefix kinship: <http://www.vberg.dev/ontologies/kinship#> .
@base <http://www.vberg.dev/ontologies/kinship#> .

<http://www.vberg.dev/ontologies/kinship#> rdf:type owl:Ontology .

#################################################################
#    Datatypes
#################################################################

###  http://www.w3.org/2001/XMLSchema#date
xsd:date rdf:type rdfs:Datatype .


#################################################################
#    Object Properties
#################################################################

###  http://www.vberg.dev/ontologies/kinship#belongsToFamily
kinship:belongsToFamily rdf:type owl:ObjectProperty ;
                        rdfs:subPropertyOf kinship:hasFamilyRelationship ;
                        owl:inverseOf kinship:hasFamilyMember ;
                        rdfs:domain kinship:Person ;
                        rdfs:range kinship:Family ;
                        rdfs:comment "Represents the relationship where a person belongs to a family."@en ;
                        rdfs:label "belongsToFamily"@en .


###  http://www.vberg.dev/ontologies/kinship#hasAdoptiveChild
kinship:hasAdoptiveChild rdf:type owl:ObjectProperty ;
                         rdfs:subPropertyOf kinship:hasChild ;
                         owl:inverseOf kinship:hasAdoptiveParent ;
                         rdfs:comment "Represents the relationship where a person has an adoptive child."@en ;
                         rdfs:label "hasAdoptiveChild"@en .


###  http://www.vberg.dev/ontologies/kinship#hasAdoptiveParent
kinship:hasAdoptiveParent rdf:type owl:ObjectProperty ;
                          rdfs:subPropertyOf kinship:hasParent ;
                          rdfs:comment "Represents the relationship where a person has an adoptive parent."@en ;
                          rdfs:label "hasAdoptiveParent"@en .


###  http://www.vberg.dev/ontologies/kinship#hasAunt
kinship:hasAunt rdf:type owl:ObjectProperty ;
                rdfs:subPropertyOf kinship:hasExtendedFamilyMember ;
                owl:inverseOf kinship:isAuntOf ;
                rdfs:domain kinship:Person ;
                rdfs:range kinship:Person ;
                rdfs:comment "Represents the relationship where an individual has an aunt (a female sibling of a parent)."@en ;
                rdfs:label "hasAunt"@en .


###  http://www.vberg.dev/ontologies/kinship#hasBiologicalChild
kinship:hasBiologicalChild rdf:type owl:ObjectProperty ;
                           rdfs:subPropertyOf kinship:hasChild ;
                           owl:inverseOf kinship:hasBiologicalParent ;
                           rdfs:comment "Represents the relationship where a person has a biological child."@en ;
                           rdfs:label "hasBiologicalChild"@en .


###  http://www.vberg.dev/ontologies/kinship#hasBiologicalParent
kinship:hasBiologicalParent rdf:type owl:ObjectProperty ;
                            rdfs:subPropertyOf kinship:hasParent ;
                            rdfs:comment "Represents the relationship where a person has a biological parent."@en ;
                            rdfs:label "hasBiologicalParent"@en .


###  http://www.vberg.dev/ontologies/kinship#hasCaretaker
kinship:hasCaretaker rdf:type owl:ObjectProperty ;
                     rdfs:subPropertyOf kinship:hasInterpersonalRelationship ;
                     rdfs:comment "Represents the relationship where a person has a caretaker."@en ;
                     rdfs:label "hasCaretaker"@en .


###  http://www.vberg.dev/ontologies/kinship#hasChild
kinship:hasChild rdf:type owl:ObjectProperty ;
                 rdfs:subPropertyOf kinship:hasInterpersonalRelationship ;
                 owl:inverseOf kinship:hasParent ;
                 rdfs:domain kinship:Person ;
                 rdfs:range kinship:Person ;
                 rdfs:comment "Represents the relationship where a person has an undefined type of child."@en ;
                 rdfs:label "hasChild"@en .


###  http://www.vberg.dev/ontologies/kinship#hasCousin
kinship:hasCousin rdf:type owl:ObjectProperty ;
                  rdfs:subPropertyOf kinship:hasExtendedFamilyMember ;
                  rdf:type owl:SymmetricProperty ;
                  rdfs:domain kinship:Person ;
                  rdfs:range kinship:Person ;
                  rdfs:comment "Represents the relationship where two individuals are cousins."@en ;
                  rdfs:label "hasCousin"@en .


###  http://www.vberg.dev/ontologies/kinship#hasExPartner
kinship:hasExPartner rdf:type owl:ObjectProperty ;
                     rdfs:subPropertyOf kinship:hasInterpersonalRelationship ;
                     rdf:type owl:SymmetricProperty ;
                     rdfs:comment "Represents a relationship where two people used to be romantically involved."@en ;
                     rdfs:label "hasExPartner"@en .


###  http://www.vberg.dev/ontologies/kinship#hasExSpouse
kinship:hasExSpouse rdf:type owl:ObjectProperty ;
                    rdfs:subPropertyOf kinship:hasExPartner ;
                    rdf:type owl:SymmetricProperty ;
                    rdfs:comment "Represents a relationship where two people used to be married."@en ;
                    rdfs:label "hasExSpouse"@en .


###  http://www.vberg.dev/ontologies/kinship#hasExtendedFamilyMember
kinship:hasExtendedFamilyMember rdf:type owl:ObjectProperty ;
                                rdfs:subPropertyOf kinship:hasInterpersonalRelationship ;
                                rdfs:comment "Represents a general relationship between a person and an extended family member, such as an aunt, uncle, or grandparent."@en ;
                                rdfs:label "hasExtendedFamilyMember"@en .


###  http://www.vberg.dev/ontologies/kinship#hasFamilyMember
kinship:hasFamilyMember rdf:type owl:ObjectProperty ;
                        rdfs:subPropertyOf kinship:hasFamilyRelationship ;
                        rdfs:domain kinship:Family ;
                        rdfs:range kinship:Person ;
                        rdfs:comment "Represents the relationship where a family has members."@en ;
                        rdfs:label "hasFamilyMember"@en .


###  http://www.vberg.dev/ontologies/kinship#hasFamilyRelationship
kinship:hasFamilyRelationship rdf:type owl:ObjectProperty ;
                              rdfs:subPropertyOf owl:topObjectProperty ;
                              rdfs:comment "Represents an unspecified relationship between a person and a family unit."@en .


###  http://www.vberg.dev/ontologies/kinship#hasFullSibling
kinship:hasFullSibling rdf:type owl:ObjectProperty ;
                       rdfs:subPropertyOf kinship:hasSibling ;
                       rdf:type owl:SymmetricProperty ;
                       rdfs:comment "Represents the relationship where two individuals share both biological parents." ;
                       rdfs:label "hasFullSibling"@en .


###  http://www.vberg.dev/ontologies/kinship#hasGrandchild
kinship:hasGrandchild rdf:type owl:ObjectProperty ;
                      rdfs:subPropertyOf kinship:hasExtendedFamilyMember ;
                      owl:inverseOf kinship:hasGrandparent ;
                      rdfs:domain kinship:Person ;
                      rdfs:range kinship:Person ;
                      rdfs:comment "Represents the relationship where a grandparent has a grandchild."@en ;
                      rdfs:label "hasGrandchild"@en .


###  http://www.vberg.dev/ontologies/kinship#hasGrandparent
kinship:hasGrandparent rdf:type owl:ObjectProperty ;
                       rdfs:subPropertyOf kinship:hasExtendedFamilyMember ;
                       rdfs:domain kinship:Person ;
                       rdfs:range kinship:Person ;
                       rdfs:comment "Represents the relationship where an individual has a grandparent."@en ;
                       rdfs:label "hasGrandparent"@en .


###  http://www.vberg.dev/ontologies/kinship#hasHalfSibling
kinship:hasHalfSibling rdf:type owl:ObjectProperty ;
                       rdfs:subPropertyOf kinship:hasSibling ;
                       rdf:type owl:SymmetricProperty ;
                       rdfs:domain kinship:Person ;
                       rdfs:range kinship:Person ;
                       rdfs:comment "Represents the relationship where two individuals share only one biological parent."@en ;
                       rdfs:label "hasHalfSibling"@en .


###  http://www.vberg.dev/ontologies/kinship#hasInterpersonalRelationship
kinship:hasInterpersonalRelationship rdf:type owl:ObjectProperty ;
                                     rdfs:subPropertyOf owl:topObjectProperty ;
                                     rdfs:domain kinship:Person ;
                                     rdfs:range kinship:Person ;
                                     rdfs:comment "Represents an undefined relationship between two people."@en ;
                                     rdfs:label "hasInterpersonalRelationship"@en .


###  http://www.vberg.dev/ontologies/kinship#hasParent
kinship:hasParent rdf:type owl:ObjectProperty ;
                  rdfs:subPropertyOf kinship:hasInterpersonalRelationship ;
                  rdfs:domain kinship:Person ;
                  rdfs:range kinship:Person ;
                  rdfs:comment "Represents the relationship where a person has an undefined type of parent."@en ;
                  rdfs:label "hasParent"@en .


###  http://www.vberg.dev/ontologies/kinship#hasPartner
kinship:hasPartner rdf:type owl:ObjectProperty ;
                   rdfs:subPropertyOf kinship:hasInterpersonalRelationship ;
                   rdf:type owl:SymmetricProperty ;
                   rdfs:comment "Represents a relationship where two people are romantically involved."@en ;
                   rdfs:label "hasPartner"@en .


###  http://www.vberg.dev/ontologies/kinship#hasSex
kinship:hasSex rdf:type owl:ObjectProperty ;
               rdfs:subPropertyOf owl:topObjectProperty ;
               rdfs:domain kinship:Person ;
               rdfs:range kinship:Sex ;
               rdfs:comment "Represents the biological sex of a person, which is typically categorized as male, female, or intersex."@en ;
               rdfs:label "hasSex" .


###  http://www.vberg.dev/ontologies/kinship#hasSibling
kinship:hasSibling rdf:type owl:ObjectProperty ;
                   rdfs:subPropertyOf kinship:hasInterpersonalRelationship ;
                   rdf:type owl:SymmetricProperty ;
                   rdfs:domain kinship:Person ;
                   rdfs:range kinship:Person ;
                   rdfs:comment "Represents the relationship where two individuals have an undefined sibling relationship.."@en ;
                   rdfs:label "hasSibling"@en .


###  http://www.vberg.dev/ontologies/kinship#hasSiblingPosition
kinship:hasSiblingPosition rdf:type owl:ObjectProperty ;
                           rdfs:subPropertyOf owl:topObjectProperty ;
                           rdfs:domain kinship:Person ;
                           rdfs:range kinship:SiblingPosition ;
                           rdfs:comment "Represents a persons sibling position."@en ;
                           rdfs:label "hasSiblingPosition"@en .


###  http://www.vberg.dev/ontologies/kinship#hasSpouse
kinship:hasSpouse rdf:type owl:ObjectProperty ;
                  rdfs:subPropertyOf kinship:hasPartner ;
                  rdf:type owl:SymmetricProperty ;
                  rdfs:domain kinship:Person ;
                  rdfs:range kinship:Person ;
                  rdfs:comment "Represents the relationship where two individuals are married."@en ;
                  rdfs:label "hasSpouse"@en .


###  http://www.vberg.dev/ontologies/kinship#hasUncle
kinship:hasUncle rdf:type owl:ObjectProperty ;
                 rdfs:subPropertyOf kinship:hasExtendedFamilyMember ;
                 owl:inverseOf kinship:isUncleOf ;
                 rdfs:domain kinship:Person ;
                 rdfs:range kinship:Person ;
                 rdfs:comment "Represents the relationship where an individual has an uncle (a male sibling of a parent)."@en ;
                 rdfs:label "hasUncle"@en .


###  http://www.vberg.dev/ontologies/kinship#isAuntOf
kinship:isAuntOf rdf:type owl:ObjectProperty ;
                 rdfs:subPropertyOf kinship:hasExtendedFamilyMember ;
                 rdfs:domain kinship:Person ;
                 rdfs:range kinship:Person ;
                 rdfs:comment "Represents the relationship where an aunt is related to a person."@en ;
                 rdfs:label "isAuntOf"@en .


###  http://www.vberg.dev/ontologies/kinship#isUncleOf
kinship:isUncleOf rdf:type owl:ObjectProperty ;
                  rdfs:subPropertyOf kinship:hasExtendedFamilyMember ;
                  rdfs:domain kinship:Person ;
                  rdfs:range kinship:Person ;
                  rdfs:comment "Represents the relationship where an uncle is related to a person."@en ;
                  rdfs:label "isUncleOf"@en .


#################################################################
#    Data properties
#################################################################

###  http://www.vberg.dev/ontologies/kinship#hasContactInformation
kinship:hasContactInformation rdf:type owl:DatatypeProperty ;
                              rdfs:subPropertyOf owl:topDataProperty .


###  http://www.vberg.dev/ontologies/kinship#hasDate
kinship:hasDate rdf:type owl:DatatypeProperty ;
                rdfs:subPropertyOf owl:topDataProperty .


###  http://www.vberg.dev/ontologies/kinship#hasDateOfBirth
kinship:hasDateOfBirth rdf:type owl:DatatypeProperty ;
                       rdfs:subPropertyOf kinship:hasDate ;
                       rdfs:domain kinship:Person ;
                       rdfs:range xsd:date ;
                       rdfs:comment "Represents the date on which a person was born."@en ;
                       rdfs:label "hasDateOfBirth"@en .


###  http://www.vberg.dev/ontologies/kinship#hasDateOfDeath
kinship:hasDateOfDeath rdf:type owl:DatatypeProperty ;
                       rdfs:subPropertyOf kinship:hasDate ;
                       rdfs:domain kinship:Person ;
                       rdfs:range xsd:date ;
                       rdfs:comment "Represents the date on which a person passed away."@en ;
                       rdfs:label "hasDateOfDeath"@en .


###  http://www.vberg.dev/ontologies/kinship#hasEmailAddress
kinship:hasEmailAddress rdf:type owl:DatatypeProperty ;
                        rdfs:subPropertyOf kinship:hasContactInformation ;
                        rdfs:domain kinship:Person ;
                        rdfs:range xsd:string ;
                        rdfs:comment "Represents the email address of a person."@en ;
                        rdfs:label "hasEmailAddress"@en .


###  http://www.vberg.dev/ontologies/kinship#hasFirstName
kinship:hasFirstName rdf:type owl:DatatypeProperty ;
                     rdfs:subPropertyOf kinship:hasName ;
                     rdfs:domain kinship:Person ;
                     rdfs:range xsd:string ;
                     rdfs:comment "Represents the first name (given name) of a person."@en ;
                     rdfs:label "hasFirstName"@en .


###  http://www.vberg.dev/ontologies/kinship#hasLastName
kinship:hasLastName rdf:type owl:DatatypeProperty ;
                    rdfs:subPropertyOf kinship:hasName ;
                    rdfs:domain kinship:Person ;
                    rdfs:range xsd:string ;
                    rdfs:comment "Represents the last name (family name or surname) of a person."@en ;
                    rdfs:label "hasLastName"@en .


###  http://www.vberg.dev/ontologies/kinship#hasName
kinship:hasName rdf:type owl:DatatypeProperty ;
                rdfs:subPropertyOf owl:topDataProperty .


###  http://www.vberg.dev/ontologies/kinship#hasNationality
kinship:hasNationality rdf:type owl:DatatypeProperty ;
                       rdfs:domain kinship:Person ;
                       rdfs:range xsd:string ;
                       rdfs:comment "Represents the nationality of a person."@en ;
                       rdfs:label "hasNationality"@en .


###  http://www.vberg.dev/ontologies/kinship#hasPhoneNumber
kinship:hasPhoneNumber rdf:type owl:DatatypeProperty ;
                       rdfs:subPropertyOf kinship:hasContactInformation ;
                       rdfs:domain kinship:Person ;
                       rdfs:range xsd:string ;
                       rdfs:comment "Represents the phone number of a person."@en ;
                       rdfs:label "hasPhoneNumber"@en .


###  http://www.vberg.dev/ontologies/kinship#hasPlaceOfBirth
kinship:hasPlaceOfBirth rdf:type owl:DatatypeProperty ;
                        rdfs:domain kinship:Person ;
                        rdfs:range xsd:string ;
                        rdfs:comment "Represents the place where a person was born."@en ;
                        rdfs:label "hasPlaceOfBirth"@en .


###  http://www.vberg.dev/ontologies/kinship#hasPlaceOfDeath
kinship:hasPlaceOfDeath rdf:type owl:DatatypeProperty ;
                        rdfs:domain kinship:Person ;
                        rdfs:range xsd:string ;
                        rdfs:comment "Represents the place where a person passed away."@en ;
                        rdfs:label "hasPlaceOfDeath"@en .


###  http://www.vberg.dev/ontologies/kinship#hasPreferredName
kinship:hasPreferredName rdf:type owl:DatatypeProperty ;
                         rdfs:subPropertyOf kinship:hasName ;
                         rdfs:domain kinship:Person ;
                         rdfs:range xsd:string ;
                         rdfs:comment "Represents the name by which a person prefers to be addressed."@en ;
                         rdfs:label "hasPreferredName"@en .


###  http://www.vberg.dev/ontologies/kinship#hasSocialSecurityNumber
kinship:hasSocialSecurityNumber rdf:type owl:DatatypeProperty ;
                                rdfs:domain kinship:Person ;
                                rdfs:range xsd:string ;
                                rdfs:comment "Represents the social security number (or equivalent identifier) of a person."@en ;
                                rdfs:label "hasSocialSecurityNumber"@en .


#################################################################
#    Classes
#################################################################

###  http://www.vberg.dev/ontologies/kinship#Enumeration
kinship:Enumeration rdf:type owl:Class ;
                    rdfs:comment "A class representing a finite set of predefined values or instances."@en ;
                    rdfs:label "Enumeration"@en .


###  http://www.vberg.dev/ontologies/kinship#Family
kinship:Family rdf:type owl:Class ;
               rdfs:subClassOf [ rdf:type owl:Restriction ;
                                 owl:onProperty kinship:hasFamilyMember ;
                                 owl:minQualifiedCardinality "2"^^xsd:nonNegativeInteger ;
                                 owl:onClass kinship:Person
                               ] ;
               rdfs:comment "Represents a family unit or group of persons related by blood, marriage, or adoption."@en ;
               rdfs:label "Family"@en .


###  http://www.vberg.dev/ontologies/kinship#Person
kinship:Person rdf:type owl:Class ;
               rdfs:subClassOf [ rdf:type owl:Restriction ;
                                 owl:onProperty kinship:belongsToFamily ;
                                 owl:minQualifiedCardinality "0"^^xsd:nonNegativeInteger ;
                                 owl:onClass kinship:Family
                               ] ,
                               [ rdf:type owl:Restriction ;
                                 owl:onProperty kinship:hasAdoptiveChild ;
                                 owl:minQualifiedCardinality "0"^^xsd:nonNegativeInteger ;
                                 owl:onClass kinship:Person
                               ] ,
                               [ rdf:type owl:Restriction ;
                                 owl:onProperty kinship:hasAdoptiveParent ;
                                 owl:minQualifiedCardinality "0"^^xsd:nonNegativeInteger ;
                                 owl:onClass kinship:Person
                               ] ,
                               [ rdf:type owl:Restriction ;
                                 owl:onProperty kinship:hasBiologicalChild ;
                                 owl:minQualifiedCardinality "0"^^xsd:nonNegativeInteger ;
                                 owl:onClass kinship:Person
                               ] ,
                               [ rdf:type owl:Restriction ;
                                 owl:onProperty kinship:hasCaretaker ;
                                 owl:minQualifiedCardinality "0"^^xsd:nonNegativeInteger ;
                                 owl:onClass kinship:Person
                               ] ,
                               [ rdf:type owl:Restriction ;
                                 owl:onProperty kinship:hasExPartner ;
                                 owl:minQualifiedCardinality "0"^^xsd:nonNegativeInteger ;
                                 owl:onClass kinship:Person
                               ] ,
                               [ rdf:type owl:Restriction ;
                                 owl:onProperty kinship:hasExSpouse ;
                                 owl:minQualifiedCardinality "0"^^xsd:nonNegativeInteger ;
                                 owl:onClass kinship:Person
                               ] ,
                               [ rdf:type owl:Restriction ;
                                 owl:onProperty kinship:hasFullSibling ;
                                 owl:minQualifiedCardinality "0"^^xsd:nonNegativeInteger ;
                                 owl:onClass kinship:Person
                               ] ,
                               [ rdf:type owl:Restriction ;
                                 owl:onProperty kinship:hasHalfSibling ;
                                 owl:minQualifiedCardinality "0"^^xsd:nonNegativeInteger ;
                                 owl:onClass kinship:Person
                               ] ,
                               [ rdf:type owl:Restriction ;
                                 owl:onProperty kinship:hasPartner ;
                                 owl:minQualifiedCardinality "0"^^xsd:nonNegativeInteger ;
                                 owl:onClass kinship:Person
                               ] ,
                               [ rdf:type owl:Restriction ;
                                 owl:onProperty kinship:hasSpouse ;
                                 owl:minQualifiedCardinality "0"^^xsd:nonNegativeInteger ;
                                 owl:onClass kinship:Person
                               ] ,
                               [ rdf:type owl:Restriction ;
                                 owl:onProperty kinship:hasBiologicalParent ;
                                 owl:qualifiedCardinality "2"^^xsd:nonNegativeInteger ;
                                 owl:onClass kinship:Person
                               ] ,
                               [ rdf:type owl:Restriction ;
                                 owl:onProperty kinship:hasSex ;
                                 owl:qualifiedCardinality "1"^^xsd:nonNegativeInteger ;
                                 owl:onClass kinship:Sex
                               ] ,
                               [ rdf:type owl:Restriction ;
                                 owl:onProperty kinship:hasSiblingPosition ;
                                 owl:qualifiedCardinality "1"^^xsd:nonNegativeInteger ;
                                 owl:onClass kinship:SiblingPosition
                               ] ,
                               [ rdf:type owl:Restriction ;
                                 owl:onProperty kinship:hasDateOfBirth ;
                                 owl:minQualifiedCardinality "0"^^xsd:nonNegativeInteger ;
                                 owl:onDataRange xsd:date
                               ] ,
                               [ rdf:type owl:Restriction ;
                                 owl:onProperty kinship:hasDateOfDeath ;
                                 owl:minQualifiedCardinality "0"^^xsd:nonNegativeInteger ;
                                 owl:onDataRange xsd:date
                               ] ,
                               [ rdf:type owl:Restriction ;
                                 owl:onProperty kinship:hasFirstName ;
                                 owl:minQualifiedCardinality "0"^^xsd:nonNegativeInteger ;
                                 owl:onDataRange xsd:string
                               ] ,
                               [ rdf:type owl:Restriction ;
                                 owl:onProperty kinship:hasNationality ;
                                 owl:minQualifiedCardinality "0"^^xsd:nonNegativeInteger ;
                                 owl:onDataRange xsd:string
                               ] ,
                               [ rdf:type owl:Restriction ;
                                 owl:onProperty kinship:hasPlaceOfBirth ;
                                 owl:minQualifiedCardinality "0"^^xsd:nonNegativeInteger ;
                                 owl:onDataRange xsd:string
                               ] ,
                               [ rdf:type owl:Restriction ;
                                 owl:onProperty kinship:hasPlaceOfDeath ;
                                 owl:minQualifiedCardinality "0"^^xsd:nonNegativeInteger ;
                                 owl:onDataRange xsd:string
                               ] ,
                               [ rdf:type owl:Restriction ;
                                 owl:onProperty kinship:hasPreferredName ;
                                 owl:minQualifiedCardinality "0"^^xsd:nonNegativeInteger ;
                                 owl:onDataRange xsd:date
                               ] ,
                               [ rdf:type owl:Restriction ;
                                 owl:onProperty kinship:hasSocialSecurityNumber ;
                                 owl:minQualifiedCardinality "0"^^xsd:nonNegativeInteger ;
                                 owl:onDataRange xsd:string
                               ] ;
               rdfs:comment "Represents an individual human being within the kinship network."@en ;
               rdfs:label "Person"@en .


###  http://www.vberg.dev/ontologies/kinship#Sex
kinship:Sex rdf:type owl:Class ;
            rdfs:subClassOf kinship:Enumeration ;
            rdfs:comment "A class representing the biological categories of sex, typically male, female, or intersex."@en ;
            rdfs:label "Sex"@en .


###  http://www.vberg.dev/ontologies/kinship#SiblingPosition
kinship:SiblingPosition rdf:type owl:Class ;
                        rdfs:subClassOf kinship:Enumeration ;
                        rdfs:comment "An enumeration class to represent a persons position in the birth order."@en ;
                        rdfs:label "SiblingPosition"@en .


#################################################################
#    Individuals
#################################################################

###  http://www.vberg.dev/ontologies/kinship#Female
kinship:Female rdf:type owl:NamedIndividual ,
                        kinship:Sex ;
               rdfs:label "Female"@en .


###  http://www.vberg.dev/ontologies/kinship#Firstborn
kinship:Firstborn rdf:type owl:NamedIndividual ,
                           kinship:SiblingPosition ;
                  rdfs:comment "Represents the firstborn child."@en ;
                  rdfs:label "Firstborn"@en .


###  http://www.vberg.dev/ontologies/kinship#Intersex
kinship:Intersex rdf:type owl:NamedIndividual ,
                          kinship:Sex ;
                 rdfs:label "Intersex"@en .


###  http://www.vberg.dev/ontologies/kinship#Male
kinship:Male rdf:type owl:NamedIndividual ,
                      kinship:Sex ;
             rdfs:label "Male"@en .


###  http://www.vberg.dev/ontologies/kinship#OnlyChild
kinship:OnlyChild rdf:type owl:NamedIndividual ,
                           kinship:SiblingPosition ;
                  rdfs:comment "Represents an only child."@en ;
                  rdfs:label "OnlyChild"@en .


###  http://www.vberg.dev/ontologies/kinship#Secondborn
kinship:Secondborn rdf:type owl:NamedIndividual ,
                            kinship:SiblingPosition ;
                   rdfs:comment "Represents the secondborn child."@en ;
                   rdfs:label "Secondborn"@en .


###  http://www.vberg.dev/ontologies/kinship#Thirdborn
kinship:Thirdborn rdf:type owl:NamedIndividual ,
                           kinship:SiblingPosition ;
                  rdfs:comment "Represents the thirdborn child."@en ;
                  rdfs:label "Thirdborn"@en .


###  http://www.vberg.dev/ontologies/kinship#Unknown
kinship:Unknown rdf:type owl:NamedIndividual ,
                         kinship:Person ,
                         kinship:Sex ,
                         kinship:SiblingPosition ;
                rdfs:label "Unknown"@en .


###  Generated by the OWL API (version 4.5.29.2024-05-13T12:11:03Z) https://github.com/owlcs/owlapi
